theories/Shallow/Gen/Synthesise.v
@@ -1,0 +1,182 @@
+(******************************************************************************)
+(* Copyright (c) 2023 Denis Carnier, Steven Keuchel                           *)
+(* All rights reserved.                                                       *)
+(*                                                                            *)
+(* Redistribution and use in source and binary forms, with or without         *)
+(* modification, are permitted provided that the following conditions are     *)
+(* met:                                                                       *)
+(*                                                                            *)
+(* 1. Redistributions of source code must retain the above copyright notice,  *)
+(*    this list of conditions and the following disclaimer.                   *)
+(*                                                                            *)
+(* 2. Redistributions in binary form must reproduce the above copyright       *)
+(*    notice, this list of conditions and the following disclaimer in the     *)
+(*    documentation and/or other materials provided with the distribution.    *)
+(*                                                                            *)
+(* THIS SOFTWARE IS PROVIDED BY THE COPYRIGHT HOLDERS AND CONTRIBUTORS        *)
+(* "AS IS" AND ANY EXPRESS OR IMPLIED WARRANTIES, INCLUDING, BUT NOT LIMITED  *)
+(* TO, THE IMPLIED WARRANTIES OF MERCHANTABILITY AND FITNESS FOR A PARTICULAR *)
+(* PURPOSE ARE DISCLAIMED. IN NO EVENT SHALL THE COPYRIGHT HOLDER OR          *)
+(* CONTRIBUTORS BE LIABLE FOR ANY DIRECT, INDIRECT, INCIDENTAL, SPECIAL,      *)
+(* EXEMPLARY, OR CONSEQUENTIAL DAMAGES (INCLUDING, BUT NOT LIMITED TO,        *)
+(* PROCUREMENT OF SUBSTITUTE GOODS OR SERVICES; LOSS OF USE, DATA, OR         *)
+(* PROFITS; OR BUSINESS INTERRUPTION) HOWEVER CAUSED AND ON ANY THEORY OF     *)
+(* LIABILITY, WHETHER IN CONTRACT, STRICT LIABILITY, OR TORT (INCLUDING       *)
+(* NEGLIGENCE OR OTHERWISE) ARISING IN ANY WAY OUT OF THE USE OF THIS         *)
+(* SOFTWARE, EVEN IF ADVISED OF THE POSSIBILITY OF SUCH DAMAGE.               *)
+(******************************************************************************)
+
+From Coq Require Import
+  Classes.Morphisms_Prop
+(*   Lists.List *)
+  Program.Tactics
+  Strings.String.
+(* From Equations Require Import *)
+(*   Equations. *)
+From stdpp Require Import
+  base gmap.
+From Em Require Import
+  Prelude
+  Shallow.Monad.Interface
+  Spec.
+
+#[local] Set Implicit Arguments.
+
+Section Elaborate.
+  Context M {mretM : MPure M} {mbindM : MBind M} {mfailM : MFail M} {tcmM : TypeCheckM M}.
+
+  Fixpoint synth (e : Exp) (Γ : Env) : M (Ty * Exp) :=
+    match e with
+    | exp.var x =>
+        match lookup x Γ with
+        | Some t => pure (t, e)
+        | None   => fail
+        end
+    | exp.false => pure (ty.bool, e)
+    | exp.true  => pure (ty.bool, e)
+    | exp.ifte e1 e2 e3 =>
+        '(t1, e1') ← synth e1 Γ;
+        '(t2, e2') ← synth e2 Γ;
+        '(t3, e3') ← synth e3 Γ;
+        equals ty.bool t1 ;;
+        equals t2 t3;;
+        pure (t3, exp.ifte e1' e2' e3')
+    | exp.absu x e =>
+        t1        ← pick;
+        '(t2, e') ← synth e (Γ ,, x∷t1);
+        pure (ty.func t1 t2, exp.abst x t1 e')
+    | exp.abst x t1 e =>
+        '(t2, e') ← synth e (Γ ,, x∷t1);
+        pure (ty.func t1 t2, exp.abst x t1 e')
+    | exp.app e1 e2 =>
+        '(tf, e1') ← synth e1 Γ;
+        '(t1, e2') ← synth e2 Γ;
+        t2         ← pick;
+        equals tf (ty.func t1 t2);;
+        pure (t2, exp.app e1' e2')
+    end.
+
+  Context {wpM : WeakestPre M} {wlpM : WeakestLiberalPre M}
+    {tclM : TypeCheckLogicM M}.
+
+  Definition tpb_algorithmic (Γ : Env) (e : Exp) (t : Ty) (ee : Exp) : Prop :=
+    WP (synth e Γ) (fun '(t',ee') => t = t' /\ ee = ee').
+  Notation "Γ |--ₐ e ∷ t ~> e'" := (tpb_algorithmic Γ e t e') (at level 80).
+
+  Ltac solve_complete :=
+    repeat
+      (rewrite ?wp_pure, ?wp_bind, ?wp_fail, ?wp_equals, ?wp_pick;
+       try
+         match goal with
+         | H: ?x = _ |- WP match ?x with _ => _ end _ => rewrite H
+         | IH: WP (synth ?Γ1 ?e) _ |- WP (synth ?Γ2 ?e) _ =>
+             unify Γ1 Γ2; revert IH; apply wp_mono; intros; subst
+         | H: _ /\ _ |- _ => destruct H; subst
+         | |- WP match ?x with _ => _ end _ =>
+             is_var x;
+             match type of x with
+             | prod Ty Exp => destruct x
+             end
+         end;
+       intros; eauto).
+
+  Lemma synth_complete (Γ : Env) (e ee : Exp) (t : Ty) :
+    Γ |-- e ∷ t ~> ee -> Γ |--ₐ e ∷ t ~> ee.
+  Proof.
+    intros T. unfold tpb_algorithmic.
+    induction T; cbn.
+    - solve_complete. now apply wp_pure.
+    - apply wp_pure. auto.
+    - apply wp_pure. auto.
+    - apply wp_bind. revert IHT1. apply wp_mono.
+      intros [t1 e1'']. intros []. subst.
+
+      apply wp_bind. revert IHT2. apply wp_mono.
+      intros [t2 e2'']. intros []. subst.
+
+      apply wp_bind. revert IHT3. apply wp_mono.
+      intros [t3 e3'']. intros []. subst.
+
+      apply wp_bind, wp_equals. split; [easy|].
+      apply wp_bind, wp_equals. split; [easy|].
+      apply wp_pure. auto.
+    - apply wp_bind.
+      eapply wp_pick with t1. intros ? <-.
+      apply wp_bind. revert IHT. apply wp_mono.
+      intros [t3 e3'']. intros []. subst.
+      apply wp_pure. auto.
+    - apply wp_bind.
+      revert IHT. apply wp_mono.
+      intros [t3 e3'']. intros []. subst.
+      apply wp_pure. auto.
+    - apply wp_bind. revert IHT1. apply wp_mono.
+      intros [tf e1'']. intros []. subst.
+      apply wp_bind. revert IHT2. apply wp_mono.
+      intros [t2' e2'']. intros []. subst.
+      apply wp_bind.
+      eapply wp_pick with t1. intros ? <-.
+      apply wp_bind, wp_equals.
+      split; auto.
+      apply wp_pure; auto.
+  (* Restart. *)
+  (*   unfold tpb_algorithmic. *)
+  (*   induction 1; cbn; solve_complete; *)
+  (*     try (eexists; solve_complete; fail). *)
+  Qed.
+
+  Lemma synth_sound (Γ : Env) (e : Exp) t ee :
+    (Γ |--ₐ e ∷ t ~> ee) -> (Γ |-- e ∷ t ~> ee).
+  Proof.
+  (*   revert Γ t ee. unfold tpb_algorithmic. *)
+  (*   induction e; cbn; intros *. *)
+  (*   4: { *)
+  (*     apply wp_bind. admit. *)
+  (*   } *)
+  (* Restart. *)
+    enough (WLP (synth e Γ) (fun '(t',ee') => Γ |-- e ∷ t' ~> ee')).
+    { unfold tpb_algorithmic. apply wp_impl. revert H.
+      apply wlp_mono. intros [t1 e1] HT [Heq1 Heq2]. now subst.
+    }
+    revert Γ. clear t ee.
+    (* induction e; cbn; intros Γ; *)
+    (*   repeat *)
+    (*     (rewrite ?wlp_ret, ?wlp_bind, ?wlp_fail, ?wlp_equals, ?wlp_pick; *)
+    (*      try *)
+    (*        match goal with *)
+    (*        | IH : forall Γ, WLP (synth Γ ?e) _ *)
+    (*          |- WLP (synth ?Γ ?e) _ => *)
+    (*          specialize (IH Γ); revert IH; apply wlp_mono; intros *)
+    (*        | |- tpb _ _ _ _    => *)
+    (*          econstructor *)
+    (*        | |- ?x = ?y -> _ => *)
+    (*          intro; subst *)
+    (*        | |- WLP (match ?t with _ => _ end) _ => *)
+    (*          destruct t eqn:? *)
+    (*        end; intros; eauto). *)
+  Admitted.
+
+  Lemma synth_correct Γ e t ee :
+    Γ |-- e ∷ t ~> ee <-> Γ |--ₐ e ∷ t ~> ee.
+  Proof. split; auto using synth_complete, synth_sound. Qed.
+
+End Elaborate.
