theories/Shallow/Monad/Free.v
@@ -1,0 +1,111 @@
+(******************************************************************************)
+(* Copyright (c) 2023 Denis Carnier, Steven Keuchel                           *)
+(* All rights reserved.                                                       *)
+(*                                                                            *)
+(* Redistribution and use in source and binary forms, with or without         *)
+(* modification, are permitted provided that the following conditions are     *)
+(* met:                                                                       *)
+(*                                                                            *)
+(* 1. Redistributions of source code must retain the above copyright notice,  *)
+(*    this list of conditions and the following disclaimer.                   *)
+(*                                                                            *)
+(* 2. Redistributions in binary form must reproduce the above copyright       *)
+(*    notice, this list of conditions and the following disclaimer in the     *)
+(*    documentation and/or other materials provided with the distribution.    *)
+(*                                                                            *)
+(* THIS SOFTWARE IS PROVIDED BY THE COPYRIGHT HOLDERS AND CONTRIBUTORS        *)
+(* "AS IS" AND ANY EXPRESS OR IMPLIED WARRANTIES, INCLUDING, BUT NOT LIMITED  *)
+(* TO, THE IMPLIED WARRANTIES OF MERCHANTABILITY AND FITNESS FOR A PARTICULAR *)
+(* PURPOSE ARE DISCLAIMED. IN NO EVENT SHALL THE COPYRIGHT HOLDER OR          *)
+(* CONTRIBUTORS BE LIABLE FOR ANY DIRECT, INDIRECT, INCIDENTAL, SPECIAL,      *)
+(* EXEMPLARY, OR CONSEQUENTIAL DAMAGES (INCLUDING, BUT NOT LIMITED TO,        *)
+(* PROCUREMENT OF SUBSTITUTE GOODS OR SERVICES; LOSS OF USE, DATA, OR         *)
+(* PROFITS; OR BUSINESS INTERRUPTION) HOWEVER CAUSED AND ON ANY THEORY OF     *)
+(* LIABILITY, WHETHER IN CONTRACT, STRICT LIABILITY, OR TORT (INCLUDING       *)
+(* NEGLIGENCE OR OTHERWISE) ARISING IN ANY WAY OUT OF THE USE OF THIS         *)
+(* SOFTWARE, EVEN IF ADVISED OF THE POSSIBILITY OF SUCH DAMAGE.               *)
+(******************************************************************************)
+
+From Coq Require Import
+  Classes.Morphisms_Prop
+(*   Lists.List *)
+  Program.Tactics
+  Strings.String.
+(* From Equations Require Import *)
+(*   Equations. *)
+From stdpp Require Import
+  base gmap.
+From Em Require Import
+  Prelude
+  Shallow.Monad.Interface
+  Spec.
+
+#[local] Set Implicit Arguments.
+
+Inductive Free (A : Type) : Type :=
+| Ret (a : A)
+| Fail
+| Equalsk (t1 t2 : Ty) (k : Free A)
+| Pickk (f : Ty -> Free A).
+#[global] Arguments Fail {A}.
+
+#[export] Instance mret_free : MPure Free :=
+  Ret.
+
+#[export] Instance mbind_free : MBind Free :=
+  fun A B =>
+    fix bind (m : Free A) f : Free B :=
+    match m with
+    | Ret a           => f a
+    | Fail            => Fail
+    | Equalsk t1 t2 k => Equalsk t1 t2 (bind k f)
+    | Pickk g       => Pickk (fun t => bind (g t) f)
+    end.
+
+#[export] Instance mfail_free : MFail Free :=
+  fun A => Fail.
+
+#[export] Instance tcm_free : TypeCheckM Free :=
+  {| equals t1 t2 := Equalsk t1 t2 (pure tt);
+    pick         := Pickk (@pure Free _ _);
+  |}.
+
+(* Eval vm_compute in *)
+(*   let e := exp.app (exp.abst "x" ty.bool (exp.var "x")) exp.true *)
+(*   in synth (M := Free) empty e. *)
+
+(* Eval vm_compute in *)
+(*   let e := exp.app (exp.absu "x" (exp.var "x")) exp.true *)
+(*   in synth (M := Free) empty e. *)
+
+(* Example K1 := exp.absu "k1" (exp.absu "l" (exp.var "k1")). *)
+(* Example K2 := exp.absu "k2" (exp.absu "l" (exp.var "k2")). *)
+(* Example I  := exp.absu "i" (exp.var "i"). *)
+
+(* Example KKI := (exp.app K1 (exp.app K2 I)). *)
+(* Eval vm_compute in *)
+(*   synth (M := Free) empty KKI. *)
+
+#[export] Instance wp_free : WeakestPre Free :=
+  fix wp [A] (m : Free A) (Q: A -> Prop) : Prop :=
+    match m with
+    | Ret a           => Q a
+    | Fail            => False
+    | Equalsk t1 t2 k => t1 = t2 /\ wp k Q
+    | Pickk f         => exists t, wp (f t) Q
+    end.
+
+#[export] Instance wlp_free : WeakestLiberalPre Free :=
+  fix wlp [A] (m : Free A) (Q: A -> Prop) : Prop :=
+    match m with
+    | Ret a           => Q a
+    | Fail            => True
+    | Equalsk t1 t2 k => t1 = t2 -> wlp k Q
+    | Pickk f         => forall t, wlp (f t) Q
+    end.
+
+#[export] Instance tcl_free: TypeCheckLogicM Free.
+Proof.
+  constructor; try (induction m; cbn; firstorder; fail); auto.
+  - cbn. intros. exists τ. auto.
+Qed.
